

Analytic Number Theory Homework 4

Xingfeng Lin

2025 Fall

1. *Proof.* Let p_n denote the n -th prime number. Then, for $\operatorname{Re}(s) > 1$,

$$\begin{aligned} s \int_2^\infty \frac{\pi(x)}{x(x^s - 1)} dx &= \sum_{n=1}^\infty n \int_{p_n}^{p_{n+1}} \frac{s}{x(x^s - 1)} dx \\ &= \sum_{n=1}^\infty n \log(1 - p_{n+1}^{-s}) - \sum_{n=1}^\infty n \log(1 - p_n^{-s}) \\ &= - \sum_{n=1}^\infty \log(1 - p_n^{-s}) \\ &= \log \zeta(s). \end{aligned}$$

□

2. In this exercise, we extend the ζ -function to \mathbb{C} and establish the Riemann's functional equation.

- (a) *Proof.* By Cauchy's theorem, we know that g is independent of ε . By definition, we have

$$2\pi i g(s) = \int_{C_{\varepsilon,1}} + \int_{C_{\varepsilon,2}} + \int_{C_{\varepsilon,3}} \frac{z^{s-1}}{e^{-z} - 1} dz.$$

Let $z = Re^{i\theta}$, then

$$\begin{aligned} g(s) &= -\frac{e^{-i\pi s}}{2\pi i} \int_\varepsilon^\infty \frac{R^{s-1}}{e^R - 1} dR + \int_{C_{\varepsilon,2}} \frac{z^{s-1}}{e^{-z} - 1} dz + \frac{e^{i\pi s}}{2\pi i} \int_\varepsilon^\infty \frac{R^{s-1}}{e^R - 1} dR \\ &= \frac{\sin \pi s}{\pi} \int_\varepsilon^\infty \frac{R^{s-1}}{e^R - 1} dR + \int_{C_{\varepsilon,2}} \frac{z^{s-1}}{e^{-z} - 1} dz. \end{aligned}$$

Note that

$$\begin{aligned} \left| \int_{C_{\varepsilon,2}} \frac{z^{s-1}}{e^{-z} - 1} dz \right| &\leq \int_{C_{\varepsilon,2}} \frac{|z^{s-1}|}{\frac{1}{2}|z|} dz \\ &\leq 4\pi \varepsilon^{\operatorname{Re}(s)-1}. \end{aligned}$$

For $\operatorname{Re}(s) > 1$, letting $\varepsilon \rightarrow 0^+$, we have

$$\lim_{\varepsilon \rightarrow 0^+} \left| \int_{C_{\varepsilon,2}} \frac{z^{s-1}}{e^{-z} - 1} dz \right| = 0$$

Therefore,

$$\begin{aligned}
g(s) &= \frac{\sin \pi s}{\pi} \int_0^\infty \frac{R^{s-1}}{e^R - 1} dR \\
&= \frac{\sin \pi s}{\pi} \int_0^\infty R^{s-1} \sum_{n=1}^\infty e^{-nR} dR \\
&= \frac{\sin \pi s}{\pi} \sum_{n=1}^\infty \int_0^\infty R^{s-1} e^{-nR} dR \\
&= \frac{\sin \pi s}{\pi} \Gamma(s) \zeta(s).
\end{aligned}$$

By Euler's reflection formula

$$\Gamma(s)\Gamma(1-s) = \frac{\pi}{\sin \pi s},$$

we have $\zeta(s) = \Gamma(1-s)g(s)$, $\operatorname{Re}(s) > 1$. □

- (b) *Proof.* Since $f_s(z) := \frac{z^{s-1}}{e^{-z}-1}$ is meromorphic inside $C_{\varepsilon,k}$, with simple poles $i2n\pi$, $n \neq 0$, by residue theorem,

$$\begin{aligned}
g_k(s) &= \sum_{n=1}^k (\operatorname{Res}(f_s, 2in\pi) + \operatorname{Res}(f_s, -2in\pi)) \\
&= \sum_{n=1}^k -(2n\pi)^{s-1} (e^{i\frac{s-1}{2}\pi} + e^{-i\frac{s-1}{2}\pi}) \\
&= 2^s \pi^{s-1} \sin(\pi s/2) \sum_{n=1}^k \frac{1}{n^{1-s}}.
\end{aligned}$$

□

- (c) *Proof.* We claim that g is an entire function. To verify this fact, it suffices to show $\int_{C_{\varepsilon,1}} \frac{z^{s-1}}{e^{-z}-1} dz$ converges locally uniformly in $s \in \mathbb{C}$, i.e. $\int_\varepsilon^\infty \frac{R^{s-1}}{e^R-1} dR$ converges locally uniformly in $s \in \mathbb{C}$. This follows from $|R^{s-1}| \lesssim_{\operatorname{Re}(s)} R^{-2}(e^R - 1)$, as $R \rightarrow +\infty$. Therefore g is holomorphic on \mathbb{C} . Recall that

$$g(s) = \frac{\sin \pi s}{\pi} \int_0^\infty \frac{R^{s-1}}{e^R - 1} dR.$$

We know g has zeros $2, 3, \dots$ of order 1. By (a) we can define the meromorphic extension of ζ on \mathbb{C} by $\zeta(s) := \Gamma(1-s)g(s)$, which is holomorphic in $\mathbb{C} - \{1\}$. To establish the functional equation of ζ , we now prove that $\lim_k g_k(s) = g(s)$, $\operatorname{Re}(s) < 0$.

Recall that $g_k(s) = \frac{1}{2\pi i} \int_{C_{\varepsilon,k}} \frac{z^{s-1}}{e^{-z}-1} dz$. Let the outer circle of $C_{\varepsilon,k}$ have radius $r_k = (2k+1)\pi$, and denote the outer circle by C_k^0 . For $z \in C_k^0$, we have $|e^z - 1| \geq C$, where $C > 0$ is independent of $z \in C_k^0$, since $\cos(r_k) = -1$. Therefore,

$$\left| \int_{C_k^0} \frac{z^{s-1}}{e^{-z}-1} dz \right| \leq \int_{-\pi}^\pi \frac{e^{\pi|\operatorname{Im}(s)|} r_k^{\operatorname{Re}(s)}}{C} d\theta \rightarrow 0,$$

as $k \rightarrow \infty$, since $\operatorname{Re}(s) > 0$, and thus we have $\lim_k g_k(s) = g(s)$, $\operatorname{Re}(s) < 0$.

From (b) we deduce that

$$g(s) = \lim_k g_k(s) = 2^s \pi^{s-1} \sin(\pi s/2) \zeta(1-s),$$

for $\operatorname{Re}(s) < 0$, and therefore,

$$\zeta(s) = 2^s \pi^{s-1} \sin(\pi s/2) \Gamma(1-s) \zeta(1-s).$$

Both sides of the equality are meromorphic functions on \mathbb{C} and agree on $\operatorname{Re}(s) < 0$, hence the equality holds for $s \in \mathbb{C}$. \square

- (d) By the functional equation we have $\zeta(-1) = -\frac{1}{12}$. One can also derive $\sum_n n = -1/12$ by nonsense calculation ignoring the divergence of the series. It is mysterious that the nonsense calculation reaches the right answer, and that this is verified in experimental physics:

the vacuum energy in a one-dimensional cavity formally contains $\frac{1}{2} \sum_n n$. If one puts the value $-1/24$ using ζ , this will lead to the Casimir force, which has been experimentally verified.

3. In this exercise we study the Laurent expansion of ζ .

- (a) *Proof.* Put $g(s) := \zeta(s) - \frac{1}{s-1}$. Then we have $\gamma_n = (-1)^n g^{(n)}(1)$. Note that

$$g(s) = 1 - s \int_1^\infty \frac{\{t\}}{t^{s+1}} dt,$$

Immediately we have $\gamma_0 = g(1) = \sum_{k=1}^\infty (\frac{1}{k} - \log(1 + \frac{1}{k}))$. For $n \geq 1$, we have

$$g^{(n)}(1) = (-1)^n \int_1^\infty \frac{\{t\} (n \log^{n-1} t - \log^n t)}{t^2} dt,$$

for $\operatorname{Re}(s) > 0$. On the other hand, We have to show that

$$\lim_{x \rightarrow +\infty} \sum_{1 \leq k \leq x} \left(\frac{\log^n k}{k} - \frac{\log^{n+1}(k+1) - \log^{n+1} k}{n+1} \right) = \int_1^\infty \frac{\{t\} (n \log^{n-1} t - \log^n t)}{t^2} dt,$$

which would complete the proof. Simplify the sum

$$\sum_{1 \leq k \leq x} \left(\frac{\log^n k}{k} - \frac{\log^{n+1}(k+1) - \log^{n+1} k}{n+1} \right) = \sum_{1 \leq k \leq x} \frac{\log^n k}{k} - \frac{1}{n+1} \log^{n+1}([x] + 1),$$

and apply Euler's summation formula, we obtain

$$\begin{aligned} \sum_{1 \leq k \leq x} \left(\frac{\log^n k}{k} - \frac{\log^{n+1}(k+1) - \log^{n+1} k}{n+1} \right) &= \int_1^x \frac{\{t\} (n \log^{n-1} t - \log^n t)}{t^2} dt \\ &\quad + \frac{\log^{n+1}(\frac{x}{[x]+1})}{n+1} + \frac{([x] - x) \log^n x}{x}. \end{aligned}$$

Letting $x \rightarrow +\infty$, we finally obtain

$$\gamma_n = \sum_{k=1}^\infty \left(\frac{\log^n k}{k} - \frac{\log^{n+1}(k+1) - \log^{n+1} k}{n+1} \right).$$

\square

- (b) *Proof.* From (a), we know that $\gamma_0 = \sum_{k=1}^{\infty} (\frac{1}{k} - \log(1 + \frac{1}{k})) = \gamma$. Therefore the Stieltjes constants are also called generalized Euler-Mascheroni constants. From the Laurent expansion, we have

$$\begin{aligned}\zeta(1 + \varepsilon) &= \frac{1}{\varepsilon} + \sum_{n=0}^{\infty} \frac{(-1)^n \gamma_n}{n!} \varepsilon^n \\ \zeta(1 - \varepsilon) &= \frac{-1}{\varepsilon} + \sum_{n=0}^{\infty} \frac{\gamma_n}{n!} \varepsilon^n,\end{aligned}$$

which gives

$$\frac{1}{2}(\zeta(1 + \varepsilon) + \zeta(1 - \varepsilon)) = \gamma_0 + \sum_{n=1}^{\infty} \frac{\gamma_{2n}}{(2n)!} \varepsilon^{2n}.$$

Letting $\varepsilon \rightarrow 0$, we obtain

$$PV[\zeta(1)] = \gamma_0.$$

□

- (c) *Proof.* By the residue theorem, we have

$$\begin{aligned}\frac{(-1)^n \gamma_n}{n!} &= \frac{1}{2\pi i} \int_C \frac{\zeta(s)}{(s-1)^{n+1}} ds \\ &= \frac{1}{2\pi} \int_0^{2\pi} \zeta(1 + e^{ix}) e^{-inx} dx,\end{aligned}$$

where C is a circle of radius 1 centered at 1. □

- (d) Here we sketch the elementary proof of the Prime Number Theorem by Selberg, 1949.

Let

$$\begin{aligned}\theta(x) &= \sum_{p \leq x} \log p \\ R(x) &= \theta(x) - x.\end{aligned}$$

Then we have the following Selberg's identity:

Theorem 1.

$$\theta(x) \log x + \sum_{p \leq x} \log p \theta\left(\frac{x}{p}\right) = 2x \log x + O(x).$$

To prove the prime number theorem, it is equivalent to prove $R(x) = o(x)$. So we have the following estimates of R :

Theorem 2.

$$R(x) \log x = \sum_{pq \leq x} \frac{\log p \log q}{\log pq} R\left(\frac{x}{pq}\right) + O(x \log \log x) \quad (1)$$

$$|R(x)| \leq \frac{1}{\log x} \sum_{n \leq x} |R\left(\frac{x}{n}\right)| + O\left(x \frac{\log \log x}{\log x}\right) \quad (2)$$

$$\sum_{n \leq x} \frac{R(n)}{n^2} = O(1). \quad (3)$$

Since $\theta(x) = O(x)$, There exist $\alpha_0 > 0$ such that $|R(x)| < \alpha x, \forall x > 1$. Theorems above will deduce that

$$|R(x)| < \alpha_0(1 - \frac{\alpha_0^2}{K})x,$$

for sufficiently large x , where K is a positive constant independent of x, α_0 . Iterate this process, we obtain a sequence $\{\alpha_n\}_{n=0}^{\infty}$ of positive real numbers satisfying

$$\alpha_{n+1} = \alpha_n(1 - \frac{\alpha_n^2}{K}),$$

and for each n , there exist some $X_n > 0$ such that $|R(x)| < \alpha_{n+1}x, \forall x > X_n$. Since $\alpha_n \rightarrow 0, n \rightarrow \infty$, We obtain

$$R(x) = o(x).$$

This completes (the sketch of) the proof of the prime number theorem.